aoc_day6/AocDay6.lean
@@ -1,3 +1,4 @@
 -- This module serves as the root of the `AocDay6` library.
 -- Import modules here that should be built as part of the library.
 import AocDay6.Grid
+import AocDay6.Thm
