aoc_day6/AocDay6/Thm.lean
@@ -1,0 +1,63 @@
+import AocDay6.Grid
+import Std.Data.HashSet.Lemmas
+
+-- To help prove termination:
+
+theorem contains_implies_non_empty (s : Std.HashSet Nat) (x : Nat) :
+    s.contains x → ¬s.isEmpty := by
+  intro h
+  false_or_by_contra
+  rename_i h'
+  have my_h : ¬x ∈ s := Std.HashSet.not_mem_of_isEmpty h'
+  contradiction
+
+theorem non_empty_implies_size_non_zero (s : Std.HashSet Nat) :
+    ¬s.isEmpty → s.size ≠ 0 := by
+  simp [Std.HashSet.isEmpty_eq_size_eq_zero]
+
+theorem erase_size_decreases (s : Std.HashSet Nat) (x : Nat) :
+    s.contains x → (s.erase x).size < s.size := by
+  intro h_contains
+  simp [Std.HashSet.size_erase]
+  have h: (if x ∈ s then s.size - 1 else s.size) = s.size - 1 := by
+    split
+    rfl
+    contradiction
+  rw [h]
+  have h_non_empty : ¬s.isEmpty := contains_implies_non_empty s x h_contains
+  have h_pos : s.size ≠ 0 := non_empty_implies_size_non_zero s h_non_empty
+  exact Nat.pred_lt h_pos
+
+-- Toy example function where the proof is analagous to the proof for our function.
+def f1 (set: Std.HashSet Nat) (n: Nat) : Option (Std.HashSet Nat) :=
+  if h: set.contains n then
+    have decrease : (set.erase n).size < set.size := erase_size_decreases set n h
+    f1 (set.erase n) (n+1)
+  else
+    none
+termination_by set.size
+
+-- For now we assume this since we proved it for Nat and it shouldn't really depend on the type.
+-- Adding it requires writing instances of LawfulBEq and LawfulHashable for Pose (and more proofs).
+theorem erase_size_decreases_pose (s : Std.HashSet Pose) (x : Pose) :
+    s.contains x → (s.erase x).size < s.size := by sorry
+
+theorem next_state_decrease_unvisited (g: Grid) (s: State) : getNextState g s = moveResults.newState s' → s'.unvisitedSet.size < s.unvisitedSet.size := by
+  intro h
+  unfold getNextState at h
+  split at h
+  simp at h
+  split at h
+  split at h
+  rename_i h_contains
+  rename_i p _
+  have h_s'_unvisited : s'.unvisitedSet = s.unvisitedSet.erase p :=
+    have h_s' : s' = {pose := p, history := p :: s.history, unvisitedSet := s.unvisitedSet.erase p} := by
+      injection h
+      rename_i h
+      rw [← h]
+    by simp [h_s']
+  rw [h_s'_unvisited]
+  exact erase_size_decreases_pose s.unvisitedSet p h_contains
+  contradiction
+  contradiction
