aoc_day6/P1.lean
@@ -4,8 +4,8 @@ import AocDay6
 
 def main : IO Unit := do
   let contents ← IO.FS.readFile "input.txt"
-  let s := readState contents
-  let reachedStates := s :: getFutureStates s
+  let (grid, s) := readState contents
+  let reachedStates := s :: getFutureStates grid s
   let futureLocs := reachedStates.map (fun s => (s.pose.x, s.pose.y))
   let uniqueFutureLocs := futureLocs.foldl (fun acc p => if acc.contains p then acc else p :: acc) []
   IO.print s!"Num unique locs : {uniqueFutureLocs.length}\n"
