aoc_day6/P2.lean
@@ -1,34 +1,37 @@
 import Init.System.FilePath
 import Init.System.IO
+import Std.Data.HashSet
 import AocDay6
 
--- TODO: prove termination
-partial def checkForCycle (s : State) : Bool :=
-  match getNextState s with
-  | .newState s' => checkForCycle s'
+def checkForCycle (grid: Grid) (s : State) : Bool :=
+  match h_match: getNextState grid s with
+  | .newState s' =>
+    have _: s'.unvisitedSet.size < s.unvisitedSet.size := next_state_decrease_unvisited grid s h_match
+    checkForCycle grid s'
   | .leftGrid => false
   | .cycle => true
+termination_by s.unvisitedSet.size
 
-def wouldAddingObstacleInduceCycle (initialState: State) (obsAddState:State) : Option (Int × Int) :=
+def wouldAddingObstacleInduceCycle (grid: Grid) (initialState: State) (obsAddState:State) : Option (Int × Int) :=
   let x := obsAddState.pose.x + obsAddState.pose.heading.toStep.fst
   let y := obsAddState.pose.y + obsAddState.pose.heading.toStep.snd
 
-  if x < 0 || x >= ((obsAddState.grid.data.get! 0).size : Int) || y < 0 || y >= (obsAddState.grid.data.size : Int) then
+  if x < 0 || x >= ((grid.data.get! 0).size : Int) || y < 0 || y >= (grid.data.size : Int) then
     none
-  else if (obsAddState.grid.getCell x y) == some '#' then
+  else if (grid.getCell x y) == some '#' then
     none
   else
-    let newGrid := {obsAddState.grid with extraObs := some (x, y)}
-    if checkForCycle {initialState with grid := newGrid} then
+    let newGrid := {grid with extraObs := some (x, y)}
+    if checkForCycle newGrid initialState then
       some (x, y)
     else
       none
 
 def main : IO Unit := do
   let contents ← IO.FS.readFile "input.txt"
-  let s := readState contents
-  let reachedStates := s :: getFutureStates s
-  let cycleOpportunities := reachedStates.map (wouldAddingObstacleInduceCycle s) |>.filterMap id
+  let (grid, s) := readState contents
+  let reachedStates := s :: getFutureStates grid s
+  let cycleOpportunities := reachedStates.map (wouldAddingObstacleInduceCycle grid s) |>.filterMap id
   let uniqueCycleOpportunities := cycleOpportunities.foldl (fun acc p => if acc.contains p then acc else p :: acc) []
   let finalCycleOpportunities := uniqueCycleOpportunities.filter (fun (x, y) => (x,y) != (s.pose.x, s.pose.y))
   IO.print s!"Num places for obstacle : {finalCycleOpportunities.length}\n"
